generic code to ext-lib & refactoring.
- Use coq-ext-lib for basic tactic automation.
- Abstract the canceler with respect to an ordering.
- Separate the unifier from the canceler and introduce
  syntactic vs semantics unification.
- Updating installation instructions.

src/SepUnify.v
@@ -6,7 +6,7 @@ Require Import List.
 Set Implicit Arguments.
 Set Strict Implicit.
 
-Module Make (U : Unifier) 
+Module Make (SUBST : Instantiation.Instantiation)
             (ST : SepTheory.SepTheory) (SE : SepExpr.SepExpr ST)
             (SH : SepHeap ST SE).
   Module SH_FACTS := SepHeapFacts ST SE SH.
@@ -14,14 +14,14 @@ Module Make (U : Unifier)
 
   Section typed.
     Variable types : list type.
-    Variable s : U.Subst types.
+    Variable s : SUBST.Subst types.
 
     Definition impuresInstantiate : MM.mmap (exprs types) -> MM.mmap (exprs types) :=
-      MM.mmap_map (map (@U.exprInstantiate _ s)).
+      MM.mmap_map (map (@SUBST.exprInstantiate _ s)).
 
     Definition sheapInstantiate (h : SH.SHeap types) : SH.SHeap types :=
       {| SH.impures := impuresInstantiate (SH.impures h)
-       ; SH.pures   := map (@U.exprInstantiate _ s) (SH.pures h)
+       ; SH.pures   := map (@SUBST.exprInstantiate _ s) (SH.pures h)
        ; SH.other   := SH.other h
        |}.
 
@@ -33,7 +33,7 @@ Module Make (U : Unifier)
     Lemma impuresInstantiate_mmap_add : forall n e acc, SE.heq funcs preds U G
         (SH.impuresD (impuresInstantiate (MM.mmap_add n e acc)))
         (SH.impuresD 
-          (MM.mmap_add n (map (@U.exprInstantiate _ s) e) 
+          (MM.mmap_add n (map (@SUBST.exprInstantiate _ s) e) 
                          (impuresInstantiate acc))).
     Proof.
       clear. intros. eapply MM.PROPS.map_induction with (m := acc); intros.
@@ -71,12 +71,12 @@ Module Make (U : Unifier)
       MM.PROPS.Add n e m m' ->
       SE.heq funcs preds U G
         (SH.impuresD (impuresInstantiate m'))
-        (SH.starred (fun v => SE.Func n (map (U.exprInstantiate s) v)) e
+        (SH.starred (fun v => SE.Func n (map (SUBST.exprInstantiate s) v)) e
           (SH.impuresD (impuresInstantiate m))).
     Proof.
       clear. intros.
         unfold impuresInstantiate, MM.mmap_map.
-        rewrite SH.impuresD_Add with (i := FM.map (map (map (U.exprInstantiate s))) m) (f := n) (argss := map (map (U.exprInstantiate s)) e).
+        rewrite SH.impuresD_Add with (i := FM.map (map (map (SUBST.exprInstantiate s))) m) (f := n) (argss := map (map (SUBST.exprInstantiate s)) e).
         symmetry; rewrite SH.starred_base. heq_canceler.
         repeat rewrite SH.starred_def.
         match goal with
@@ -92,21 +92,21 @@ Module Make (U : Unifier)
     Qed.
 
     Lemma applyD_forget_exprInstantiate :
-      U.Subst_equations funcs U G s ->
+      SUBST.Subst_equations funcs U G s ->
       forall D R F l,
-        applyD (exprD funcs U G) D (map (U.exprInstantiate s) l) R F =
+        applyD (exprD funcs U G) D (map (SUBST.exprInstantiate s) l) R F =
         applyD (exprD funcs U G) D l R F.
     Proof.
       clear. induction D; destruct l; simpl; auto.
-      rewrite U.Subst_equations_exprInstantiate; eauto.
+      rewrite SUBST.Subst_equations_exprInstantiate; eauto.
       destruct (exprD funcs U G e a); eauto.
     Qed.
 
     Lemma starred_forget_exprInstantiate : forall x P,
-      U.Subst_equations funcs U G s ->
+      SUBST.Subst_equations funcs U G s ->
       forall e,
       SE.heq funcs preds U G 
-        (SH.starred (fun v : list (expr types) => SE.Func x (map (U.exprInstantiate s) v)) e P)
+        (SH.starred (fun v : list (expr types) => SE.Func x (map (SUBST.exprInstantiate s) v)) e P)
         (SH.starred (SE.Func x) e P).
     Proof.
       clear. induction e; intros; repeat rewrite SH.starred_def; simpl; repeat rewrite <- SH.starred_def; SEP_FACTS.heq_canceler.
@@ -120,7 +120,7 @@ Module Make (U : Unifier)
     Qed.
 
     Lemma impuresD_forget_impuresInstantiate : forall h,
-      U.Subst_equations funcs U G s ->
+      SUBST.Subst_equations funcs U G s ->
       SE.heq funcs preds U G 
         (SH.impuresD (impuresInstantiate h))
         (SH.impuresD h).
@@ -133,8 +133,8 @@ Module Make (U : Unifier)
     Qed.
 
     Lemma Func_forget_exprInstantiate : forall n e,
-      U.Subst_equations funcs U G s ->
-      SE.heq funcs preds U G (SE.Func n (map (U.exprInstantiate s) e)) (SE.Func n e).
+      SUBST.Subst_equations funcs U G s ->
+      SE.heq funcs preds U G (SE.Func n (map (SUBST.exprInstantiate s) e)) (SE.Func n e).
     Proof. clear.
       unfold SE.heq. simpl. intros.
       destruct (nth_error preds n); try reflexivity.
