src/ExprUnifySyn.v
@@ -1,0 +1,390 @@
+Require Import List Bool.
+Require Import Expr.
+Require Import ExprUnify.
+Require Import Instantiation.
+
+Module SynUnifier (S : Instantiation) <: SyntacticUnifier S.
+  Require Import NatMap.
+
+  Section typed.
+    Variable types : list type.
+
+    Section unify.
+      Variable exprUnify : expr types -> expr types -> S.Subst types -> option (S.Subst types).      
+
+      Fixpoint unify (l r : expr types) (sub : S.Subst types) : option (S.Subst types) :=
+        match l , r with
+          | Const t v , Const t' v' => 
+            match equiv_dec t t' with
+              | left pf => match pf in _ = k return tvarD _ k -> _ with
+                             | refl_equal => fun v' =>
+                               if get_Eq types t v v'
+                                 then Some sub
+                                 else None
+                           end v'
+              | right _ => None
+            end
+          | Var v , Var v' => 
+            if Peano_dec.eq_nat_dec v v' 
+              then Some sub
+              else None
+          | Func f1 args1 , Func f2 args2 =>
+            if EqNat.beq_nat f1 f2 then
+              (fix unifyArgs (args1 args2 : list (expr types)) (s : S.Subst types) 
+                : option (S.Subst types) :=
+                match args1 , args2 with
+                  | nil , nil => Some s
+                  | nil , _ :: _ => None
+                  | _ :: _ , nil => None
+                  | arg1 :: args1 , arg2 :: args2 =>
+                    match unify arg1 arg2 s with
+                      | None => None
+                      | Some s => unifyArgs args1 args2 s
+                    end
+                end) args1 args2 sub
+              else None
+          | Equal t1 e1 f1 , Equal t2 e2 f2 =>
+            if equiv_dec t1 t2 then
+              match unify e1 e2 sub with
+                | None => None
+                | Some sub => unify f1 f2 sub
+              end
+              else
+                None
+          | Not e1 , Not e2 =>
+            unify e1 e2 sub
+          | UVar l , UVar r => 
+            if EqNat.beq_nat l r then Some sub
+              else 
+                match S.Subst_lookup l sub with
+                  | None => S.Subst_set l (UVar r) sub
+                  | Some l' =>
+                    match S.Subst_lookup r sub with
+                      | None => S.Subst_set r l' sub
+                      | Some r' =>
+                        exprUnify l' r' sub
+                    end
+                end
+          | UVar u , r =>
+            match S.Subst_lookup u sub with
+              | None =>
+                S.Subst_set u r sub
+              | Some l' =>
+                exprUnify l' r sub
+            end
+          | l , UVar u =>
+            match S.Subst_lookup u sub with
+              | None => 
+                S.Subst_set u l sub
+              | Some r' =>
+                exprUnify l r' sub
+            end
+          | _ , _ => None
+        end.
+    End unify.
+
+    Fixpoint exprUnify (bound : nat) : expr types -> expr types -> (S.Subst types) -> option (S.Subst types) :=
+      match bound with 
+        | 0 => fun _ _ _ => None
+        | S bound =>
+          fix unify (l r : expr types) (sub : S.Subst types) : option (S.Subst types) :=
+            match l , r with
+              | Const t v , Const t' v' => 
+                match equiv_dec t t' with
+                  | left pf => match pf in _ = k return tvarD _ k -> _ with
+                                 | refl_equal => fun v' =>
+                                   if get_Eq types t v v'
+                                     then Some sub
+                                     else None
+                               end v'
+                  | right _ => None
+                end
+            | Var v , Var v' => 
+              if EqNat.beq_nat v v' 
+                then Some sub
+                else None
+            | Func f1 args1 , Func f2 args2 =>
+              if EqNat.beq_nat f1 f2 then
+                (fix unifyArgs (args1 args2 : list (expr types)) (s : S.Subst types) 
+                  : option (S.Subst types) :=
+                  match args1 , args2 with
+                    | nil , nil => Some s
+                    | nil , _ :: _ => None
+                    | _ :: _ , nil => None
+                    | arg1 :: args1 , arg2 :: args2 =>
+                      match unify arg1 arg2 s with
+                        | None => None
+                        | Some s => unifyArgs args1 args2 s
+                      end
+                  end) args1 args2 sub
+              else None
+            | Equal t1 e1 f1 , Equal t2 e2 f2 =>
+              if equiv_dec t1 t2 then
+                match unify e1 e2 sub with
+                  | None => None
+                  | Some sub => unify f1 f2 sub
+                end
+              else
+                None
+            | Not e1 , Not e2 =>
+              unify e1 e2 sub
+            | UVar l , UVar r => 
+              if EqNat.beq_nat l r then Some sub
+              else 
+                match S.Subst_lookup l sub with
+                  | None => S.Subst_set l (UVar r) sub
+                  | Some l' =>
+                    match S.Subst_lookup r sub with
+                      | None => S.Subst_set r l' sub
+                      | Some r' =>
+                        exprUnify bound l' r' sub
+                    end
+                end
+            | UVar u , r =>
+              match S.Subst_lookup u sub with
+                | None =>
+                  S.Subst_set u r sub
+                | Some l' =>
+                  exprUnify bound l' r sub
+              end
+            | l , UVar u =>
+              match S.Subst_lookup u sub with
+                | None => 
+                  S.Subst_set u l sub
+                | Some r' =>
+                  exprUnify bound l r' sub
+              end
+            | _ , _ => None
+            end
+      end.
+
+    Hint Rewrite S.exprInstantiate_Func S.exprInstantiate_Equal S.exprInstantiate_Not 
+      S.exprInstantiate_UVar S.exprInstantiate_Var S.exprInstantiate_Const : subst_simpl.
+
+    Opaque S.Subst_lookup S.Subst_set S.exprInstantiate.
+
+    Require Import ExtLib.Tactics.Consider.
+
+    Theorem unify_uvar : forall (u : uvar) (sub sub' : S.Subst types)
+      (o : expr types -> expr types -> S.Subst types -> option (S.Subst types)),
+      (forall (l r : expr types) (sub0 sub'0 : S.Subst types),
+        o l r sub0 = Some sub'0 ->
+        S.exprInstantiate sub'0 l = S.exprInstantiate sub'0 r /\
+        S.Subst_Extends sub'0 sub0 /\
+        (forall (funcs : tfunctions) (U G : tenv) (t : tvar),
+          is_well_typed funcs U G l t = true ->
+          is_well_typed funcs U G r t = true ->
+          S.Subst_WellTyped funcs U G sub0 -> S.Subst_WellTyped funcs U G sub'0)) ->
+      forall e : expr types,
+        match S.Subst_lookup u sub with
+          | Some r' => o e r' sub
+          | None => S.Subst_set u e sub
+        end = Some sub' ->
+        S.exprInstantiate sub' e = S.exprInstantiate sub' (UVar u) /\
+        S.Subst_Extends sub' sub /\
+        (forall (funcs : tfunctions) (U G : tenv) (t1 : tvar),
+          is_well_typed funcs U G e t1 = true ->
+          is_well_typed (types := types) funcs U G (UVar u) t1 = true ->
+          S.Subst_WellTyped funcs U G sub -> S.Subst_WellTyped funcs U G sub').
+    Proof.
+      intros. consider (S.Subst_lookup u sub); intros.
+      { specialize (H _ _ _ _ H1). rewrite S.exprInstantiate_UVar.
+        intuition.
+        { erewrite S.Subst_lookup_Extends by eassumption. auto. }
+        { eapply H4; try eassumption.
+          destruct (S.WellTyped_lookup H6 H0). intuition. simpl in H5.
+          rewrite H8 in *.
+          destruct (nth_error U u); try congruence.
+          consider (tvar_seqb t1 x); congruence. } }
+      { clear H; intuition. 
+        { erewrite S.Subst_set_exprInstantiate by eassumption; auto. }
+        { eapply S.Subst_set_Extends; eauto. }
+        { eapply S.Subst_set_WellTyped; try eassumption. simpl in H2.
+          destruct (nth_error U u); try congruence.
+          consider (tvar_seqb t1 t); congruence. } }
+    Qed.
+
+    Lemma exprUnify_all : forall n l r sub sub',
+      exprUnify n l r sub = Some sub' ->
+         (S.exprInstantiate sub' l = S.exprInstantiate sub' r)
+      /\ (S.Subst_Extends sub' sub)
+      /\ (forall funcs U G t,
+            is_well_typed funcs U G l t = true ->
+            is_well_typed funcs U G r t = true ->
+            S.Subst_WellTyped funcs U G sub ->
+            S.Subst_WellTyped funcs U G sub').
+    Proof.
+      induction n; simpl in *; try congruence.
+      induction l; simpl in *.
+      { destruct r; simpl in *; intros; try congruence.
+        { consider (equiv_dec t t1); unfold equiv in *; simpl in *; intros; subst; try congruence.
+          consider (get_Eq types t1 t0 t2); try congruence; simpl in *; intros.
+          inversion H0; clear H0; subst. split; [ reflexivity | split; [ reflexivity | ] ].
+          intros. consider (tvar_seqb t1 t); intros; subst; auto. }
+        { eapply unify_uvar; eauto. } }
+      { destruct r; simpl in *; intros; try congruence.
+        { consider (EqNat.beq_nat x v); try congruence; subst; intros.
+          inversion H0; clear H0; subst. intuition. }
+        { eapply unify_uvar; eauto. } }
+      { do 4 intro.
+        assert ((exists u, r = UVar u) \/
+                match S.Subst_lookup x sub with
+                  | Some l' => exprUnify n l' r sub
+                  | None => S.Subst_set x r sub
+                end = Some sub').
+        { destruct r; auto. left. eauto. }
+        destruct H0.
+        { destruct H0; subst.
+          consider (EqNat.beq_nat x x0); intros; subst.
+          { inversion H0; clear H0; subst. intuition. }
+          { consider (S.Subst_lookup x sub); intros.
+            { consider (S.Subst_lookup x0 sub); intros.
+              { repeat rewrite S.exprInstantiate_UVar.
+                specialize (IHn _ _ _ _ H2). destruct IHn as [ ? [ ? ? ] ].
+                repeat erewrite S.Subst_lookup_Extends by eassumption.
+                intuition. 
+                simpl in *; consider (nth_error U x); consider (nth_error U x0); intros.
+                consider (tvar_seqb t t0); consider (tvar_seqb t t1); intros.
+                subst. subst.
+                destruct (S.WellTyped_lookup H8 H0).
+                destruct (S.WellTyped_lookup H8 H1).
+                rewrite H6 in *. rewrite H9 in *.
+                intuition. inversion H11; inversion H7; subst. subst.
+                eapply H5; eauto. } 
+              { intuition.
+                { erewrite S.Subst_set_exprInstantiate with (x := x0) by eassumption.
+                  rewrite S.exprInstantiate_UVar.
+                  erewrite S.Subst_lookup_Extends; try eassumption.
+                  reflexivity. eapply S.Subst_set_Extends; eauto. }
+                { eapply S.Subst_set_Extends; eauto. }
+                { simpl in *. 
+                  consider (nth_error U x); consider (nth_error U x0); intros.
+                  consider (tvar_seqb t t0); consider (tvar_seqb t t1); intros; subst.
+                  eapply S.Subst_set_WellTyped; try eassumption.
+                  subst.
+                  destruct (S.WellTyped_lookup H5 H0); intuition.
+                  rewrite H6 in *. inversion H7. subst. auto. } } }
+            { intuition.
+              { erewrite S.Subst_set_exprInstantiate with (x := x) by eassumption. 
+                reflexivity. }
+              { eapply S.Subst_set_Extends; eauto. }
+              { simpl in *. 
+                consider (nth_error U x); consider (nth_error U x0); intros.
+                consider (tvar_seqb t t0); consider (tvar_seqb t t1); intros; subst.
+                eapply S.Subst_set_WellTyped; try eassumption.
+                subst. simpl. rewrite H2. consider (tvar_seqb t0 t0); auto. } } } } 
+        { clear H. consider (S.Subst_lookup x sub); intros.
+          { specialize (IHn _ _ _ _ H0); intuition.
+            { rewrite S.exprInstantiate_UVar. 
+              erewrite S.Subst_lookup_Extends; try eassumption. }
+            { eapply H4; try eassumption.
+              destruct (S.WellTyped_lookup H6 H). 
+              destruct (nth_error U x); try congruence.
+              intuition. inversion H8; clear H8; subst.
+              consider (tvar_seqb t x0); try congruence. } }
+          { intuition. 
+            { erewrite S.Subst_set_exprInstantiate by eassumption. auto. }
+            { eapply S.Subst_set_Extends; eauto. }
+            { eapply S.Subst_set_WellTyped; eauto.
+              destruct (nth_error U x); try congruence.
+              consider (tvar_seqb t t0); try congruence. } } } }
+      { destruct r; simpl in *; intros; try congruence.
+        { consider (EqNat.beq_nat f f0); try congruence; intros; subst.
+          intros. apply and_assoc. 
+          split.
+          { generalize dependent l0; generalize dependent sub; generalize dependent sub'.
+            induction H.
+            { destruct l0; try congruence. inversion 1; subst. intuition. }
+            { destruct l0; try congruence; intros.
+              match goal with
+                | [ H : match ?X _ _ _ with _ => _ end = _ |- _ ] =>
+                  generalize dependent X; intros
+              end.
+              consider (o x e sub); try congruence; intros.
+              specialize (H _ _ _ H1). specialize (IHForall _ _ _ H2). clear H2.
+              intuition.
+              { simpl. inversion H; clear H; subst.
+                repeat rewrite S.exprInstantiate_Func in *.
+                simpl. f_equal. inversion H7; f_equal; auto.
+                erewrite <- S.exprInstantiate_Extends with (y := s); eauto. rewrite H2.
+                rewrite S.exprInstantiate_Extends; auto. }
+              { etransitivity; eauto. } } }
+          { intros. destruct (nth_error funcs f0); try congruence.
+            destruct t0. simpl in *.
+            generalize dependent l0; generalize dependent sub; generalize dependent sub'; 
+              generalize dependent TDomain.
+            induction H.
+            { destruct l0; try congruence. } (*inversion 1; subst. 
+              destruct (tvar_seqb t TRange); try congruence. auto. } *)
+            { destruct l0; try congruence. intros.
+              match goal with
+                | [ H : match ?X _ _ _ with _ => _ end = _ |- _ ] =>
+                  generalize dependent X; intros
+              end.
+              consider (o x e sub); intros; try congruence.
+              specialize (H _ _ _ H2).
+              consider (tvar_seqb t TRange); intros; subst. simpl in *.
+              destruct TDomain; try congruence.
+              consider (is_well_typed funcs U G x t).
+              consider (is_well_typed funcs U G e t).
+              intuition. eapply H7. 3: eapply H5. eassumption. eauto. eauto. } } }
+        { eapply unify_uvar; eauto. } }
+      { destruct r; intros; try congruence.
+        { consider (equiv_dec t t0); try congruence; unfold equiv in *; simpl in *; intros; subst.
+          match goal with
+            | [ H : match ?X _ _ _ with _ => _ end = _ |- _ ] =>
+              generalize dependent X; intros
+          end.
+          consider (o l1 r1 sub); try congruence; intros.
+          specialize (IHl1 _ _ _ H). specialize (IHl2 _ _ _ H0).
+          intuition.
+          { do 2 rewrite S.exprInstantiate_Equal. f_equal; auto. 
+            erewrite <- S.exprInstantiate_Extends with (y := s); eauto. rewrite H1.
+            rewrite S.exprInstantiate_Extends; auto. }
+          { etransitivity; eauto. }
+          { destruct t; try congruence.
+            eapply andb_true_iff in H4. eapply andb_true_iff in H8. intuition eauto. } }
+        { eapply unify_uvar; eauto. } }
+      { destruct r; intros; try congruence.
+        { specialize (IHl _ _ _ H). clear H. intuition eauto. 
+          repeat rewrite S.exprInstantiate_Not. rewrite H. auto.
+          destruct t; try congruence. simpl in *. eauto. } 
+        { eapply unify_uvar; eauto. } }
+    Qed.
+
+    Theorem exprUnify_sound_syn : forall n l r sub sub',
+      exprUnify n l r sub = Some sub' ->
+      S.exprInstantiate sub' l = S.exprInstantiate sub' r.
+    Proof.
+      intros. specialize (exprUnify_all _ _ _ _ _ H); intuition.
+    Qed.
+
+    Theorem exprUnify_sound_sem : forall n l r sub sub',
+      exprUnify n l r sub = Some sub' ->
+      forall funcs U G t,
+      exprD funcs U G (S.exprInstantiate sub' l) t = 
+      exprD funcs U G (S.exprInstantiate sub' r) t.
+    Proof.
+      intros. f_equal. specialize (exprUnify_all _ _ _ _ _ H); intuition. 
+    Qed.
+
+    Theorem exprUnify_Extends : forall n l r sub sub',
+      exprUnify n l r sub = Some sub' ->
+      S.Subst_Extends sub' sub.
+    Proof.
+      intros. specialize (exprUnify_all _ _ _ _ _ H); intuition.
+    Qed.
+
+    Theorem exprUnify_WellTyped : forall n l r sub sub',
+      exprUnify n l r sub = Some sub' ->
+      forall funcs U G t,
+        is_well_typed funcs U G l t = true ->
+        is_well_typed funcs U G r t = true ->
+        S.Subst_WellTyped funcs U G sub ->
+        S.Subst_WellTyped funcs U G sub'.
+    Proof.
+      do 6 intro. specialize (exprUnify_all _ _ _ _ _ H); intuition.
+    Qed.
+
+  End typed.
+End SynUnifier.
