src/ListFacts.v
@@ -1,7 +1,7 @@
 Require Import List.
 Require Import Omega.
 Require Import Tactics.
-Require Import Reflection.
+Require Import ExtLib.Tactics.Consider.
 
 Lemma skipn_length_gt : forall T (ls : list T) n,
   length ls <= n ->
