src/OrderedCanceler.v
@@ -1,0 +1,1136 @@
+Require Import List.
+Require Import Folds Tactics.
+Require Import ExtLib.Tactics.Consider.
+Require Import Instantiation ExprUnify.
+Require Import Expr SepExpr SepHeap SepCancel.
+Require Import Prover.
+
+Set Implicit Arguments.
+Set Strict Implicit.
+
+Module Type Ordering (ST : SepTheory.SepTheory)
+                     (SE : SepExpr ST)
+                     (SH : SepHeap ST SE).
+
+  Section typed.
+    Variable types : list type.
+
+    Parameter order_impures : MM.mmap (exprs types) -> list (exprs types * nat).
+
+    Parameter meta_order_args : exprs types -> exprs types -> Datatypes.comparison.
+    
+    Parameter meta_order_funcs : (exprs types * func) -> (exprs types * func) -> Datatypes.comparison.
+    
+    Axiom order_impures_D : forall funcs preds U G imps,
+      SE.heq funcs preds U G 
+            (SH.impuresD imps)
+            (SH.starred (fun v => (SE.Func (snd v) (fst v))) (order_impures imps) SE.Emp).
+
+    Axiom order_impures_WellTyped : forall tf tp tU tG imp,
+      SH.WellTyped_impures tf tp tU tG imp = true ->
+      allb (fun v : list (expr types) * func => SE.WellTyped_sexpr tf tp tU tG
+        (SE.Func (snd v) (fst v))) (order_impures imp) = true.
+  End typed.
+End Ordering.
+
+Lemma allb_permutation : forall T F (a b : list T),
+  Permutation.Permutation a b ->
+  allb F a = allb F b.
+Proof. clear.
+  induction 1; simpl; auto.
+  destruct (F x); auto.
+  destruct (F x); destruct (F y); auto.
+  rewrite IHPermutation1; auto.
+Qed.
+
+Module DefaultOrdering (ST : SepTheory.SepTheory)
+                       (SE : SepExpr ST)
+                       (SH : SepHeap ST SE) <: Ordering ST SE SH.
+
+  Module HEAP_FACTS := SepHeapFacts ST SE SH.
+  Module Import SEP_FACTS := HEAP_FACTS.SEP_FACTS.
+  
+  Section typed.
+    Variable types : list type.
+
+    (** This function determines whether an expression [l] is more "defined"
+     ** than an expression [r]. An expression is more defined if it "uses UVars later".
+     ** NOTE: This is a "fuzzy property" but correctness doesn't depend on it.
+     **)
+    Fixpoint expr_count_meta (e : expr types) : nat :=
+      match e with
+        | Expr.Const _ _
+        | Var _ => 0
+        | UVar _ => 1
+        | Not l => expr_count_meta l
+        | Equal _ l r => expr_count_meta l + expr_count_meta r
+        | Expr.Func _ args =>
+          fold_left plus (map expr_count_meta args) 0
+      end.
+
+    Fixpoint exprs_count_meta (es : exprs types) : nat :=
+      match es with
+        | nil => O
+        | e :: es' => expr_count_meta e + exprs_count_meta es'
+      end.
+
+    (** When expressions have the same number of uvars, we want to favor the larger
+     ** expressions first, since they are less likely to match spuriously. *)
+    Fixpoint expr_size (e : expr types) : nat :=
+      match e with
+        | Expr.Const _ _
+        | Var _
+        | UVar _ => 0
+        | Not l => S (expr_size l)
+        | Equal _ l r => S (expr_size l + expr_size r)
+        | Expr.Func _ args => fold_left plus (map expr_size args) 1
+      end.
+
+    Definition meta_order_args (l r : exprs types) : Datatypes.comparison :=
+      match Compare_dec.nat_compare (exprs_count_meta l) (exprs_count_meta r) with
+        | Datatypes.Eq =>
+          Ordering.list_lex_cmp _ (fun l r => Compare_dec.nat_compare (expr_size l) (expr_size r)) l r
+        | v => v
+      end.
+
+    Definition meta_order_funcs (l r : exprs types * func) : Datatypes.comparison :=
+      match snd l, snd r with
+        | 2, 0 => Datatypes.Lt
+        | 2, 1 => Datatypes.Lt
+        | 2, S (S (S _)) => Datatypes.Lt
+        | _, _ =>
+          match meta_order_args (fst l) (fst r) with
+            | Datatypes.Eq => Compare_dec.nat_compare (snd l) (snd r)
+            | x => x
+          end
+      end.
+
+    Definition order_impures (imps : MM.mmap (exprs types)) : list (exprs types * nat) :=
+      FM.fold (fun k => fold_left (fun (acc : list (exprs types * nat)) (args : exprs types) => 
+        Ordering.insert_in_order _ meta_order_funcs (args, k) acc)) imps nil.
+
+    Lemma impuresD'_flatten : forall funcs preds U G imps,
+      SE.heq funcs preds U G
+        (SH.impuresD imps)
+        (SH.starred (fun v => SE.Func (snd v) (fst v)) 
+          (FM.fold (fun f argss acc => 
+            map (fun args => (args, f)) argss ++ acc) imps nil) (@SE.Emp types)).
+    Proof.
+      clear. intros. eapply MM.PROPS.fold_rec; intros.
+      { rewrite (SH.impuresD_Empty funcs preds U G H).
+        rewrite SH.starred_def. simpl. reflexivity. }
+
+      { rewrite SH.impuresD_Add; eauto. rewrite SH.starred_app. 
+        rewrite H2. symmetry. rewrite SH.starred_base. heq_canceler.
+        repeat rewrite SH.starred_def.
+        clear; induction e; simpl; intros; try reflexivity.
+        rewrite IHe. reflexivity. }
+    Qed.
+
+    Lemma fold_Permutation : forall imps L R,
+      Permutation.Permutation L R ->
+      Permutation.Permutation
+      (FM.fold (fun (f : FM.key) (argss : list (exprs types)) (acc : list (exprs types * FM.key)) =>
+        map (fun args : exprs types => (args, f)) argss ++ acc) imps L)
+      (FM.fold
+        (fun k : FM.key =>
+         fold_left
+           (fun (acc : list (exprs types * nat)) (args : exprs types) =>
+            Ordering.insert_in_order (exprs types * nat) meta_order_funcs
+              (args, k) acc)) imps R).
+    Proof.
+      clear. intros.
+      eapply @MM.PROPS.fold_rel; simpl; intros; auto.
+        revert H1; clear. revert a; revert b; induction e; simpl; intros; auto.
+        rewrite <- IHe; eauto.
+        
+        destruct (@Ordering.insert_in_order_inserts (exprs types * nat) meta_order_funcs (a,k) b) as [ ? [ ? [ ? ? ] ] ].
+        subst. rewrite H.
+        rewrite <- app_ass.
+        eapply Permutation.Permutation_cons_app.
+        rewrite app_ass. eapply Permutation.Permutation_app; eauto.
+    Qed.
+
+    Lemma order_impures_D : forall funcs preds U G imps,
+      SE.heq funcs preds U G 
+        (SH.impuresD imps)
+        (SH.starred (fun v => (SE.Func (snd v) (fst v))) (order_impures imps) SE.Emp).
+    Proof.
+      clear. intros. rewrite impuresD'_flatten. unfold order_impures.
+      eapply SH.starred_perm. eapply fold_Permutation. reflexivity.
+    Qed.
+
+    Lemma fold_left_insert_perm : forall e a k,
+      Permutation.Permutation (map (fun x => (x,k)) e ++ a)
+      (fold_left
+        (fun (acc : list (exprs types * nat)) (args : exprs types) =>
+          Ordering.insert_in_order (exprs types * func) meta_order_funcs
+          (args, k) acc) e a).
+    Proof.
+      clear. induction e; simpl.
+      eauto.
+      intros. rewrite <- IHe; clear IHe.
+      destruct (@Ordering.insert_in_order_inserts _ meta_order_funcs (a,k) a0). destruct H.
+      intuition subst. rewrite H0.
+      rewrite <- app_ass. rewrite <- app_ass.
+      eapply Permutation.Permutation_middle.
+    Qed.
+
+    Lemma fold_left_fold_left_insert_perm : forall l (B : list (exprs types * nat)),
+      Permutation.Permutation 
+      (B ++ fold_left (fun (a : list (exprs types * nat)) (p : FM.key * list (list (expr types))) =>
+        fold_left (fun (acc : list (exprs types * nat)) (args : list (expr types)) =>
+          Ordering.insert_in_order (list (expr types) * func) meta_order_funcs (args, fst p) acc) (snd p) a) l nil)
+      (fold_left (fun (a : list (exprs types * nat)) (p : FM.key * list (list (expr types))) =>
+        fold_left (fun (acc : list (exprs types * nat)) (args : list (expr types)) =>
+          Ordering.insert_in_order (list (expr types) * func) meta_order_funcs (args, fst p) acc) (snd p) a) l B).
+    Proof.
+      induction l; simpl; intros. 
+      rewrite app_nil_r; reflexivity.
+      etransitivity. 2: eapply IHl. destruct a; simpl. 
+      symmetry. 
+      rewrite Permutation.Permutation_app_tail.
+      2: symmetry; apply (@fold_left_insert_perm l0 B k).
+      rewrite Permutation.Permutation_app_tail.
+      2: apply Permutation.Permutation_app_comm with (l' := B). rewrite app_ass.
+      apply Permutation.Permutation_app_head.
+      etransitivity. 2: eapply IHl. apply Permutation.Permutation_app_tail.
+      etransitivity. 2: apply fold_left_insert_perm. rewrite app_nil_r; auto.
+    Qed.
+
+    Lemma order_impures_WellTyped : forall tf tp tU tG imp,
+      SH.WellTyped_impures tf tp tU tG imp = true ->
+      allb (fun v : list (expr types) * func => SE.WellTyped_sexpr tf tp tU tG
+        (SE.Func (snd v) (fst v))) (order_impures imp) = true.
+    Proof. clear.
+      intros. unfold order_impures.
+      rewrite SH.WellTyped_impures_spec_eq in H.
+      rewrite FM.fold_1 in *. revert H. unfold exprs in *. generalize true at 2 4.
+      induction (FM.elements (elt:=list (list (expr types))) imp); auto; intros.
+      simpl in *. 
+      assert (fold_left
+        (fun (a : bool) (p : FM.key * list (list (expr types))) =>
+          (a &&
+            match snd p with
+              | nil => true
+              | _ :: _ =>
+                match nth_error tp (fst p) with
+                  | Some ts =>
+                    allb
+                    (fun args : list (expr types) =>
+                      all2
+                      (is_well_typed tf
+                        tU tG) args ts) 
+                    (snd p)
+                  | None => false
+                end
+            end)%bool) l false = false).
+      { clear. induction l; simpl; auto. } 
+      destruct b; simpl in H; try congruence.
+      destruct a. destruct l0; simpl in *. eauto.
+      consider (nth_error tp k); intros; try congruence.
+      consider (all2 (is_well_typed tf tU tG) l0 t); intros; try congruence.
+      consider (allb
+        (fun args : list (expr types) =>
+          all2
+          (is_well_typed tf tU tG) args t) l1); intros; try congruence.
+      rewrite <- IHl by assumption.
+      erewrite allb_permutation. 
+      2: symmetry; apply fold_left_fold_left_insert_perm.
+      rewrite allb_app. erewrite <- allb_permutation.
+      2: eapply fold_left_insert_perm.
+      rewrite allb_app. rewrite allb_map. simpl. unfold exprs in *.
+      think. simpl. auto. 
+    Qed.
+
+  End typed.
+End DefaultOrdering.
+
+Module Make (SUBST : Instantiation)
+            (U : SyntacticUnifier SUBST)
+            (ST : SepTheory.SepTheory)
+            (Import SE : SepExpr ST)
+            (SH : SepHeap ST SE)
+            (O : Ordering ST SE SH)
+  <: Canceller SUBST ST SE SH.
+
+  Module HEAP_FACTS := SepHeapFacts ST SE SH.
+  Module Import SEP_FACTS := HEAP_FACTS.SEP_FACTS.
+  Import HEAP_FACTS.
+  Module Import SEP_UFACTS := SepUnify.Make SUBST ST SE SH.
+
+  Section env.
+    Variable types : list type.
+
+    Variable funcs : functions types.
+    Variable preds : SE.predicates types.
+
+    (** The actual tactic code **)
+    Variable Prover : ProverT types.
+    Variable Prover_correct : ProverT_correct Prover funcs.
+
+    Definition unifyArgs (bound : nat) (summ : Facts Prover) (l r : list (expr types)) (ts : list tvar) (sub : SUBST.Subst types)
+      : option (SUBST.Subst types) :=
+      Folds.fold_left_3_opt 
+        (fun l r t (acc : SUBST.Subst _) =>
+          if Prove Prover summ (Expr.Equal t (SUBST.exprInstantiate acc l) (SUBST.exprInstantiate acc r))
+            then Some acc
+            else U.exprUnify bound l r acc)
+        l r ts sub.
+
+    Fixpoint unify_remove (bound : nat) (summ : Facts Prover) (l : exprs types) (ts : list tvar) (r : list (exprs types))
+      (sub : SUBST.Subst types)
+      : option (list (list (expr types)) * SUBST.Subst types) :=
+        match r with 
+          | nil => None
+          | a :: b => 
+            match unifyArgs bound summ l a ts sub with
+              | None => 
+                match unify_remove bound summ l ts b sub with
+                  | None => None
+                  | Some (x,sub) => Some (a :: x, sub)
+                end
+              | Some sub => Some (b, sub)
+            end
+        end.
+    
+    Section with_typing.
+      Variable tfuncs : tfunctions.
+      Variables tU tG : tenv.
+      Variables U G : env types.
+
+      Hypothesis WT_funcs : WellTyped_funcs tfuncs funcs.
+      Hypothesis WT_env_U : WellTyped_env tU U.
+      Hypothesis WT_env_G : WellTyped_env tG G.
+
+      Lemma unifyArgs_Extends_WellTyped : forall bound summ l r ts S S',
+        SUBST.Subst_WellTyped tfuncs tU tG S ->
+        all2 (@is_well_typed _ tfuncs tU tG) l ts = true ->
+        all2 (@is_well_typed _ tfuncs tU tG) r ts = true ->
+        unifyArgs bound summ l r ts S = Some S' ->
+        SUBST.Subst_Extends S' S /\
+        SUBST.Subst_WellTyped tfuncs tU tG S'.
+      Proof.
+        unfold unifyArgs; induction l; destruct r; destruct ts; simpl; intros; try congruence.
+        { inversion H2. subst; intuition; auto. }
+        { repeat match goal with
+          | [ H : (if ?X then _ else _) = true |- _ ] =>
+            revert H; case_eq X; intros; [ | congruence ]
+                   | [ |- context [ exprD ?A ?B ?C ?D ?E ] ] =>
+                     case_eq (exprD A B C D E); intros
+                 end; simpl in *;
+        try solve [ 
+          match goal with
+            | [ H : is_well_typed _ _ _ ?e _ = true , H' : exprD _ _ _ (SUBST.exprInstantiate ?S' ?e) _ = None |- _ ] =>
+              exfalso; revert H; revert H'; clear; intros H' H;
+                eapply WellTyped_exprInstantiate with (S := S') in H;
+                  eapply is_well_typed_correct in H;
+                    rewrite H' in H ; destruct H; congruence
+          end ].
+          consider (Prove Prover summ (Equal t (SUBST.exprInstantiate S a) (SUBST.exprInstantiate S e))); simpl; eauto.
+          consider (U.exprUnify bound a e S); intros; try congruence.
+          eapply IHl in H6; eauto using U.exprUnify_WellTyped.
+          intuition. etransitivity; eauto using U.exprUnify_Extends. }
+      Qed.          
+
+      Lemma unifyArgs_bad_cases : forall summ bound S S' ts t e a l r,
+        SUBST.Subst_WellTyped tfuncs tU tG S ->
+        all2 (@is_well_typed _ tfuncs tU tG) l ts = true ->
+        all2 (@is_well_typed _ tfuncs tU tG) r ts = true ->
+        @is_well_typed _ tfuncs tU tG a t = true ->
+        @is_well_typed _ tfuncs tU tG e t = true ->
+        match
+          (if Prove Prover summ
+            (Equal t (SUBST.exprInstantiate S a) (SUBST.exprInstantiate S e))
+            then Some S
+            else U.exprUnify bound a e S)
+          with
+          | Some acc =>
+            fold_left_3_opt
+            (fun (l r : expr types) (t : tvar) (acc0 : SUBST.Subst types) =>
+              if Prove Prover summ
+                (Equal t (SUBST.exprInstantiate acc0 l)
+                  (SUBST.exprInstantiate acc0 r))
+                then Some acc0
+                else U.exprUnify bound l r acc0) l r ts acc
+          | None => None
+        end = Some S' ->
+        SUBST.Subst_Extends S' S /\ SUBST.Subst_WellTyped tfuncs tU tG S'.
+      Proof.
+        intros. destruct (Prove Prover summ (Equal t (SUBST.exprInstantiate S a) (SUBST.exprInstantiate S e))).
+        apply unifyArgs_Extends_WellTyped in H4; eauto; intuition.
+        revert H4. case_eq (U.exprUnify bound a e S); intros; eauto.
+        generalize H4. eapply U.exprUnify_Extends in H4.
+        intro. eapply U.exprUnify_WellTyped in H6; eauto.
+        eapply unifyArgs_Extends_WellTyped in H5; eauto; intuition.
+        etransitivity; eauto. 
+        congruence.
+      Qed.
+
+      Lemma unifyArgsOk : forall bound summ R l r ts f S S',
+        SUBST.Subst_WellTyped tfuncs tU tG S ->
+        Valid Prover_correct U G summ ->
+        all2 (@is_well_typed _ tfuncs tU tG) l ts = true ->
+        all2 (@is_well_typed _ tfuncs tU tG) r ts = true ->
+        unifyArgs bound summ l r ts S = Some S' ->
+        SUBST.Subst_equations funcs U G S' ->
+        @applyD types (exprD funcs U G) ts (map (SUBST.exprInstantiate S') l) R f =
+        @applyD types (exprD funcs U G) ts (map (SUBST.exprInstantiate S') r) R f /\
+        SUBST.Subst_Extends S' S /\
+        SUBST.Subst_WellTyped tfuncs tU tG S'.
+      Proof.
+        unfold unifyArgs; induction l; destruct r; destruct ts; simpl; intros; try congruence.
+        { inversion H2. inversion H3; subst; intuition; auto. }
+        { repeat match goal with
+          | [ H : (if ?X then _ else _) = true |- _ ] =>
+            revert H; case_eq X; intros; [ | congruence ]
+                   | [ |- context [ exprD ?A ?B ?C ?D ?E ] ] =>
+                     case_eq (exprD A B C D E); intros
+                 end; simpl in *;
+        try solve [ 
+          match goal with
+            | [ H : is_well_typed _ _ _ ?e _ = true , H' : exprD _ _ _ (SUBST.exprInstantiate ?S' ?e) _ = None |- _ ] =>
+              exfalso; revert H; revert H'; clear; intros H' H;
+                eapply WellTyped_exprInstantiate with (S := S') in H;
+                  eapply is_well_typed_correct in H;
+                    rewrite H' in H ; destruct H; congruence
+          end ].
+          revert H3. case_eq (Prove Prover summ (Equal t (SUBST.exprInstantiate S a) (SUBST.exprInstantiate S e))); intros.
+          { eapply Prove_correct in H3; eauto.
+            erewrite SUBST.exprInstantiate_WellTyped in H2 by eauto.
+            erewrite SUBST.exprInstantiate_WellTyped in H1 by eauto.
+            eapply is_well_typed_correct in H2; eauto.
+            eapply is_well_typed_correct in H1; eauto.
+            destruct H2; destruct H1.
+            unfold ValidProp, Provable in *. simpl in *.
+            repeat match goal with 
+                     | [ H : _ = _ |- _ ] => rewrite H in *
+                     | [ H : ?X -> ?Y |- _ ] => 
+                       let H' := fresh in assert (H':X) by eauto; specialize (H H')
+                   end.
+            subst.
+            eapply IHl with (f := f t0) in H9; eauto.
+            intuition. rewrite H3. f_equal. f_equal.
+            erewrite <- SUBST.Subst_equations_exprInstantiate in H2 by eauto.
+            erewrite <- SUBST.Subst_equations_exprInstantiate in H1 by eauto.
+            rewrite SUBST.exprInstantiate_Extends in H2 by eauto.
+            rewrite SUBST.exprInstantiate_Extends in H1 by eauto.
+            rewrite H2 in H8. rewrite H1 in H7. inversion H7; inversion H8; subst; auto. }
+          { clear H3. revert H9. case_eq (U.exprUnify bound a e S); intros; try congruence.
+            eapply IHl with (f := f t0) in H9; eauto using U.exprUnify_WellTyped.
+            intuition.
+            rewrite H10. f_equal. f_equal.
+            eapply U.exprUnify_sound_sem with (funcs := funcs) (U := U) (G := G) (t := t) in H3.
+            generalize H9. 
+            eapply SUBST.exprInstantiate_Extends with (t := a) in H9.
+            intro.
+            eapply SUBST.exprInstantiate_Extends with (t := e) in H11.
+            rewrite <- H9 in H7.
+            rewrite <- H11 in H8.
+            rewrite SUBST.Subst_equations_exprInstantiate in H7 by eassumption.
+            rewrite SUBST.Subst_equations_exprInstantiate in H8 by eassumption.
+            rewrite H3 in H7. rewrite H7 in H8. inversion H8; auto.
+
+            etransitivity; eauto using U.exprUnify_Extends. }
+          { exfalso.
+            eapply unifyArgs_bad_cases in H3; eauto; intuition.
+            do 2 match goal with
+              | [ H : is_well_typed _ _ _ ?E _ = true ,
+                  H' : exprD _ _ _ ?E _ = None |- _ ] =>
+              (eapply is_well_typed_correct in H ; eauto) ; destruct H; congruence
+              | [ H : exprD _ _ _ ?E _ = None |- _ ] =>
+                assert (@is_well_typed _ tfuncs tU tG E t = true) by 
+                  (rewrite <- SUBST.exprInstantiate_WellTyped; eauto)
+            end. }
+          { exfalso.
+            eapply unifyArgs_bad_cases in H3; eauto; intuition.
+            do 2 match goal with
+              | [ H : is_well_typed _ _ _ ?E _ = true ,
+                  H' : exprD _ _ _ ?E _ = None |- _ ] =>
+              (eapply is_well_typed_correct in H ; eauto) ; destruct H; congruence
+              | [ H : exprD _ _ _ ?E _ = None |- _ ] =>
+                assert (@is_well_typed _ tfuncs tU tG E t = true) by 
+                  (rewrite <- SUBST.exprInstantiate_WellTyped; eauto)
+            end. }
+          { exfalso.
+            eapply unifyArgs_bad_cases in H3; eauto; intuition.
+            do 2 match goal with
+              | [ H : is_well_typed _ _ _ ?E _ = true ,
+                  H' : exprD _ _ _ ?E _ = None |- _ ] =>
+              (eapply is_well_typed_correct in H ; eauto) ; destruct H; congruence
+              | [ H : exprD _ _ _ ?E _ = None |- _ ] =>
+                assert (@is_well_typed _ tfuncs tU tG E t = true) by 
+                  (rewrite <- SUBST.exprInstantiate_WellTyped; eauto)
+            end. } }
+      Qed.
+      
+      Lemma unify_removeOk : forall bound summ f p l S,
+        SUBST.Subst_WellTyped tfuncs tU tG S ->
+        Valid Prover_correct U G summ ->
+        nth_error preds f = Some p ->
+        all2 (@is_well_typed _ tfuncs tU tG) l (SE.SDomain p) = true ->
+        forall r r' S' P,
+          List.Forall (fun r => all2 (@is_well_typed _ tfuncs tU tG) r (SE.SDomain p) = true) r ->
+          unify_remove bound summ l (SE.SDomain p) r S = Some (r', S') ->
+          SUBST.Subst_equations funcs U G S' ->
+          forall Q,
+          SE.himp funcs preds U G (SH.starred (SE.Func f) r' Q) P ->
+          SE.himp funcs preds U G
+            (SH.starred (SE.Func f) r Q) (SE.Star (SE.Func f l) P) /\
+          SUBST.Subst_Extends S' S.
+      Proof.
+        induction r; simpl; intros; try congruence.
+        revert H4. case_eq (unifyArgs bound summ l a (SDomain p) S); intros; try congruence.
+        { inversion H7; clear H7; subst.
+          inversion H3; clear H3; subst.
+          rewrite SH.starred_def. simpl. rewrite <- SH.starred_def.
+          eapply unifyArgsOk with (R := ST.hprop) (f := SDenotation p) in H4;
+            eauto. 
+          intuition.
+          apply himp_star_frame; auto. unfold himp; simpl. rewrite H1.
+          match goal with
+            | [ |- ST.himp match ?X with _ => _ end match ?Y with _ => _ end ] =>
+              cutrewrite (X = Y)
+          end. reflexivity.
+          revert H3. repeat rewrite applyD_forget_exprInstantiate by eauto; eauto. }
+        { revert H7. case_eq (unify_remove bound summ l (SDomain p) r S); intros; try congruence.
+          destruct p0. inversion H8; clear H8; subst. clear H4.
+          inversion H3; clear H3; subst.
+          rewrite SH.starred_def in H6. simpl in H6. rewrite <- SH.starred_def in H6.
+          eapply IHr in H7; eauto.
+          Focus 2. instantiate (2 := (SE.Star (Func f a) Q)). instantiate (1 := P).
+          etransitivity; [ | eapply H6 ].
+          rewrite SH.starred_base. rewrite heq_star_assoc. 
+          rewrite SH.starred_base with (base := Q). reflexivity.
+          intuition. rewrite starred_cons. rewrite <- H3. 
+          rewrite SH.starred_base. rewrite SH.starred_base with (base := SE.Star (Func f a) Q). 
+          rewrite heq_star_assoc. reflexivity. }
+      Qed.
+
+      Lemma unify_remove_PureFacts : forall bound summ f p l S,
+        SUBST.Subst_WellTyped tfuncs tU tG S ->
+        nth_error preds f = Some p ->
+        all2 (@is_well_typed _ tfuncs tU tG) l (SDomain p) = true ->
+        forall r r' S',
+          List.Forall (fun r => all2 (@is_well_typed _ tfuncs tU tG) r (SDomain p) = true) r ->
+          unify_remove bound summ l (SDomain p) r S = Some (r', S') ->
+             SUBST.Subst_Extends S' S
+          /\ SUBST.Subst_WellTyped tfuncs tU tG S'
+          /\ List.Forall (fun r => all2 (@is_well_typed _ tfuncs tU tG) r (SDomain p) = true) r'.
+      Proof.
+        induction r; simpl; intros; try congruence.
+        consider (unifyArgs bound summ l a (SDomain p) S); intros.
+        { inversion H4; clear H4; subst. inversion H2; clear H2; subst.
+          eapply unifyArgs_Extends_WellTyped in H3; eauto. intuition eauto. }
+        { consider (unify_remove bound summ l (SDomain p) r S); intros.
+          { destruct p0. inversion H5; clear H5; subst. inversion H2; clear H2; subst.
+            eapply IHr in H8; intuition. eauto. eauto. eauto. }
+          { congruence. } }
+      Qed.
+
+    End with_typing.
+
+    Definition cancel_list : Type := list (exprs types * nat).
+    
+    (** NOTE : l and r are reversed here **)
+    (** cancel_in_order ls acc rem = (l,r,sub) ->
+     ** r ===> l ->
+     ** rem ===> ls * acc
+     **)
+    Fixpoint cancel_in_order (bound : nat) (summ : Facts Prover) (tpreds : SE.tpredicates)
+      (ls : cancel_list) (acc rem : MM.mmap (exprs types)) (sub : SUBST.Subst types)
+      (progress : bool)
+      : option (MM.mmap (exprs types) * MM.mmap (exprs types) * SUBST.Subst types) :=
+      match ls with
+        | nil => 
+          if progress then Some (acc, rem, sub) else None
+        | (args,f) :: ls => 
+          match FM.find f rem with
+            | None => cancel_in_order bound summ tpreds ls (MM.mmap_add f args acc) rem sub progress
+            | Some argss =>
+              match nth_error tpreds f with
+                | None => cancel_in_order bound summ tpreds ls (MM.mmap_add f args acc) rem sub progress (** Unused! **)
+                | Some ts => 
+                  match unify_remove bound summ args ts argss sub with
+                    | None => cancel_in_order bound summ tpreds ls (MM.mmap_add f args acc) rem sub progress
+                    | Some (rem', sub) =>
+                      cancel_in_order bound summ tpreds ls acc (FM.add f rem' rem) sub true
+                  end
+              end                      
+          end
+      end.
+
+    Lemma cancel_in_order_equiv : forall bound summ tpreds ls acc rem sub L R S acc' progress,
+      MM.mmap_Equiv acc acc' ->
+      cancel_in_order bound summ tpreds ls acc rem sub progress = Some (L, R, S) ->
+      exists L' R' S',
+        cancel_in_order bound summ tpreds ls acc' rem sub progress = Some (L', R', S') /\
+        MM.mmap_Equiv L L' /\
+        MM.mmap_Equiv R R' /\
+        SUBST.Subst_Equal S S'.
+    Proof.
+      clear. induction ls; simpl; intros.
+      { inversion H0; subst; auto. 
+        destruct progress; try congruence. inversion H0; clear H0; subst.
+        do 3 eexists. split; [ reflexivity | intuition ]. }
+      { repeat match goal with
+                 | [ H : match ?X with 
+                           | (_,_) => _
+                         end = _ |- _ ] => destruct X
+                 | [ H : match ?X with
+                           | Some _ => _ | None => _ 
+                         end = _ |- _ ] =>
+                 revert H; case_eq X; intros
+               end;
+        (eapply IHls; [ eauto using MM.mmap_add_mor | eassumption ]). }
+    Qed.
+
+    Lemma cancel_in_order_mmap_add_acc : forall bound summ tpreds ls n e acc rem sub L R S progress,
+      cancel_in_order bound summ tpreds ls (MM.mmap_add n e acc) rem sub progress = Some (L, R, S) ->
+      exists L' R' S',
+        cancel_in_order bound summ tpreds ls acc rem sub progress = Some (L', R', S') /\
+        MM.mmap_Equiv (MM.mmap_add n e L') L /\
+        MM.mmap_Equiv R R' /\
+        SUBST.Subst_Equal S S'.
+    Proof.
+      clear. induction ls; simpl; intros.
+      { inversion H; subst.
+        destruct progress; try congruence. inversion H; clear H; subst.
+        do 3 eexists; split. 
+        reflexivity. split; try reflexivity. split; try reflexivity. }
+      { repeat match goal with
+                 | [ H : match ?X with 
+                           | (_,_) => _
+                         end = _ |- _ ] => destruct X
+                 | [ H : match ?X with
+                           | Some _ => _ | None => _ 
+                         end = _ |- _ ] =>
+                 revert H; case_eq X; intros
+               end;
+        try solve [ eapply IHls; eauto ];
+        match goal with
+          | [ H : cancel_in_order _ _ _ _ _ _ _ _ = _ |- _ ] =>
+            eapply cancel_in_order_equiv in H; [ | eapply MM.mmap_add_comm ]
+        end;
+        repeat match goal with
+                 | [ H : exists x, _ |- _ ] => destruct H
+                 | [ H : _ /\ _ |- _ ] => destruct H
+               end;
+        match goal with
+          | [ H : cancel_in_order _ _ _ _ _ _ _ _ = _ |- _ ] =>
+            eapply IHls in H
+        end;
+        repeat match goal with
+                 | [ H : exists x, _ |- _ ] => destruct H
+                 | [ H : _ /\ _ |- _ ] => destruct H
+                 | [ |- exists x, _ /\ _ ] => eexists; split; [ eassumption | ]
+                 | [ |- exists x, _ ] => eexists
+                 | [ H : MM.mmap_Equiv _ _ |- _ ] => rewrite H
+                 | [ H : SUBST.Subst_Equal _ _ |- _ ] => rewrite H
+               end; try intuition reflexivity. }
+    Qed.
+
+    Lemma nth_error_typeof_preds : forall p n,
+      nth_error (typeof_preds p) n = option_map (@typeof_pred types) (nth_error p n).
+    Proof.
+      clear. unfold typeof_preds. intros. rewrite Tactics.map_nth_error_full. reflexivity.
+    Qed.
+
+    Lemma WellTyped_impures_add : forall tf tp tU tG f l m,
+      SH.WellTyped_impures (types := types) tf tp tU tG m = true ->
+      match nth_error tp f with
+        | None => false
+        | Some p => allb (fun l => all2 (is_well_typed tf tU tG) l p) l
+      end = true ->
+      SH.WellTyped_impures tf tp tU tG (FM.add f l m) = true.
+    Proof. clear.
+      intros. eapply SH.WellTyped_impures_eq. intros.
+      consider (nth_error tp f); try congruence; intros.
+      rewrite MF.FACTS.add_o in H1. destruct (MF.FACTS.eq_dec f k); think.
+      destruct v; auto.
+      eapply SH.WellTyped_impures_eq in H; eauto.
+    Qed.
+
+    Lemma WellTyped_impures_mmap_add : forall tf tp tU tG f l m,
+      SH.WellTyped_impures (types := types) tf tp tU tG m = true ->
+      match nth_error tp f with
+        | None => false
+        | Some p => all2 (is_well_typed tf tU tG) l p
+      end = true ->
+      SH.WellTyped_impures tf tp tU tG (MM.mmap_add f l m) = true.
+    Proof. clear.
+      intros. eapply SH.WellTyped_impures_eq. intros.
+      consider (nth_error tp f); try congruence; intros.
+      unfold MM.mmap_add in *. consider (FM.find (elt:=list (list (expr types))) f m); intros.
+      rewrite MF.FACTS.add_o in H3. destruct (MF.FACTS.eq_dec f k).
+      { inversion H3; clear H3; subst. rewrite H0. simpl. rewrite H2.
+        eapply SH.WellTyped_impures_eq in H. 2: eauto. destruct l0; auto. rewrite H0 in *. assumption. }
+      { eapply SH.WellTyped_impures_eq; eauto. }
+      { rewrite MF.FACTS.add_o in H3. destruct (MF.FACTS.eq_dec f k).
+        inversion H3; clear H3; subst. rewrite H0. simpl; rewrite H2; auto.
+        eapply SH.WellTyped_impures_eq; eauto. }
+    Qed.
+
+    Lemma cancel_in_order_PureFacts_weak : forall tU tG bound summ,
+      let tf := typeof_funcs funcs in
+      let tp := SE.typeof_preds preds in
+(*
+      let tU := typeof_env U in
+      let tG := typeof_env G in *)
+      forall ls acc rem sub L R S progress,
+      SUBST.Subst_WellTyped tf tU tG sub ->
+      allb (fun v => SE.WellTyped_sexpr tf tp tU tG 
+        (Func (snd v) (fst v))) ls = true ->
+      SH.WellTyped_impures tf tp tU tG acc = true ->
+      SH.WellTyped_impures tf tp tU tG rem = true ->
+(*      Valid Prover_correct U G summ ->  *)
+      cancel_in_order bound summ tp ls acc rem sub progress = Some (L, R, S) ->
+         SUBST.Subst_Extends S sub 
+      /\ SUBST.Subst_WellTyped tf tU tG S
+      /\ SH.WellTyped_impures tf tp tU tG L = true 
+      /\ SH.WellTyped_impures tf tp tU tG R = true.
+    Proof.
+      induction ls; simpl; intros.
+      { destruct progress; try congruence. inversion H3; clear H3; subst; intuition. }
+      { subst tp. rewrite nth_error_typeof_preds in H0. destruct a; simpl in *. 
+        repeat match goal with
+                 | H : context [ option_map _ ?X ] |- _ =>
+                   (consider X; simpl in *; try congruence); [ intros ]
+                 | [ H : match ?X with _ => _ end = _ |- _ ] =>
+                   (consider X; intros; try congruence); [ intros ]
+                 | [ H : match ?X with
+                           | Some _ => _ | None => _ 
+                         end = _ |- _ ] =>
+                 consider X; intros
+               end; simpl in *; subst.
+        { assert (List.Forall
+          (fun r : list (expr types) =>
+            all2 (is_well_typed tf tU tG) r (SDomain p) = true) l0).
+          { eapply SH.WellTyped_impures_eq in H2; try eassumption.
+            destruct l0. constructor. rewrite nth_error_typeof_preds in H2.
+            rewrite H0 in H2. generalize dependent (e :: l0); simpl; intros.
+            unfold typeof_pred in H2. clear - H2.
+            induction l2; simpl in *; constructor; think; auto. }
+          eapply unify_remove_PureFacts in H7.
+          2: eauto. 2: eauto. 2: eauto.
+          Focus 2. cutrewrite (SDomain p = t); eauto.
+          unfold typeof_preds in H6.
+          rewrite map_nth_error_full in H6. rewrite H0 in *.
+          inversion H6. auto.
+          { eapply IHls in H9; eauto. intuition.
+            etransitivity. eapply H10. eapply H9.
+            intuition. intuition.
+            eapply SH.WellTyped_impures_eq. intros. rewrite MF.FACTS.add_o in H11.
+            destruct (MF.FACTS.eq_dec f k); auto. inversion H11; clear H11; subst. 
+            rewrite nth_error_typeof_preds in *. rewrite H0 in *. simpl. destruct v; intuition.
+            generalize dependent (e :: v); intros.
+            clear - H12. unfold typeof_pred. induction H12; simpl; auto. rewrite H. auto.
+            eapply SH.WellTyped_impures_eq; eauto. } }
+        { clear H6. eapply IHls in H8; eauto.
+          eapply WellTyped_impures_mmap_add; auto. rewrite nth_error_typeof_preds.
+          rewrite H0. simpl. auto. }
+        { eapply IHls in H7; eauto.
+          eapply WellTyped_impures_mmap_add; auto. rewrite nth_error_typeof_preds.
+          rewrite H0. simpl. auto. }
+        { eapply IHls in H6; eauto.
+          eapply WellTyped_impures_mmap_add; auto. rewrite nth_error_typeof_preds.
+          rewrite H0. simpl. auto. } }
+    Qed.
+
+    Lemma cancel_in_order_PureFacts : forall U G bound summ,
+      let tf := typeof_funcs funcs in
+      let tp := SE.typeof_preds preds in
+      let tU := typeof_env U in
+      let tG := typeof_env G in
+      forall ls acc rem sub L R S progress,
+      SUBST.Subst_WellTyped tf tU tG sub ->
+      SUBST.Subst_equations funcs U G S ->
+      allb (fun v => SE.WellTyped_sexpr tf tp tU tG 
+        (Func (snd v) (fst v))) ls = true ->
+      SH.WellTyped_impures tf tp tU tG acc = true ->
+      SH.WellTyped_impures tf tp tU tG rem = true ->
+      cancel_in_order bound summ tp ls acc rem sub progress = Some (L, R, S) ->
+         SUBST.Subst_equations funcs U G sub 
+      /\ SUBST.Subst_WellTyped (typeof_funcs funcs) (typeof_env U) (typeof_env G) S
+      /\ SH.WellTyped_impures tf tp tU tG L = true 
+      /\ SH.WellTyped_impures tf tp tU tG R = true.
+    Proof.
+      intros.
+      eapply cancel_in_order_PureFacts_weak in H4; try eassumption. intuition.
+      eapply SUBST.Subst_equations_Extends. 2: eassumption. eauto. 
+    Qed.
+
+    Lemma impuresD_mmap_add : forall U G f args m,
+      heq funcs preds U G 
+          (SH.impuresD (MM.mmap_add f args m))
+          (Star (Func f args) (SH.impuresD m)).
+    Proof. clear.
+      intros. unfold MM.mmap_add. consider (FM.find (elt:=list (exprs types)) f m); intros.
+      { rewrite SH.impuresD_Add with (f := f) (argss := args :: l) (i := FM.remove f m).
+        rewrite starred_cons. 
+        rewrite SH.impuresD_Add with (f := f) (argss := l) (i := FM.remove f m) (i' := m).
+        heq_canceler.
+        intro. repeat (rewrite MF.FACTS.add_o || rewrite MF.FACTS.remove_o). destruct (MF.FACTS.eq_dec f y); subst; auto.
+        rewrite MF.FACTS.remove_in_iff. intro. intuition; congruence.
+        intro. repeat (rewrite MF.FACTS.add_o || rewrite MF.FACTS.remove_o). destruct (MF.FACTS.eq_dec f y); subst; auto.
+        rewrite MF.FACTS.remove_in_iff. intro. intuition; congruence. }
+      { rewrite SH.impuresD_Add with (f := f) (argss := args :: nil) (i := m).
+        rewrite starred_cons. 
+        heq_canceler.
+        intro. repeat (rewrite MF.FACTS.add_o || rewrite MF.FACTS.remove_o). destruct (MF.FACTS.eq_dec f y); subst; auto.
+        intro. destruct H0. apply MF.FACTS.find_mapsto_iff in H0; congruence. }
+    Qed.
+
+    Lemma cancel_in_order_common : forall 
+      (U G : env types)
+      (bound : nat) (summ : Facts Prover) (e : exprs types) 
+      (n : nat) (ls : list (exprs types * nat)),
+      (forall (acc rem : MM.mmap (exprs types)) (sub : SUBST.Subst types)
+        (L R : MM.mmap (exprs types)) (S : SUBST.Subst types) progress,
+        SUBST.Subst_WellTyped (typeof_funcs funcs) (typeof_env U) (typeof_env G) sub ->
+        SUBST.Subst_WellTyped (typeof_funcs funcs) (typeof_env U) (typeof_env G) S ->
+        SUBST.Subst_equations funcs U G S ->
+        Valid Prover_correct U G summ ->
+        cancel_in_order bound summ (SE.typeof_preds preds) ls acc rem sub progress = Some (L, R, S) ->
+        allb
+        (fun v : list (expr types) * func =>
+          match nth_error (typeof_preds preds) (snd v) with
+            | Some ts =>
+              all2
+              (is_well_typed (typeof_funcs funcs) (typeof_env U)
+                (typeof_env G)) (map (SUBST.exprInstantiate S) (fst v)) ts
+            | None => false
+          end) ls = true ->
+        SH.WellTyped_impures (typeof_funcs funcs) (typeof_preds preds)
+        (typeof_env U) (typeof_env G) acc = true ->
+        SH.WellTyped_impures (typeof_funcs funcs) (typeof_preds preds)
+        (typeof_env U) (typeof_env G) rem = true ->
+        forall P Q,
+          himp funcs preds U G
+          (Star (SH.impuresD (impuresInstantiate S R)) P)
+          (Star (SH.impuresD (impuresInstantiate S L)) Q) ->
+          himp funcs preds U G
+          (Star (SH.impuresD (impuresInstantiate S rem)) P)
+          (Star
+            (Star
+              (SH.starred
+                (fun v : list (expr types) * func =>
+                  Func (snd v) (map (SUBST.exprInstantiate S) (fst v))) ls Emp)
+              (SH.impuresD (impuresInstantiate S acc))) Q)) ->
+      forall (acc rem : MM.mmap (exprs types)) (sub : SUBST.Subst types)
+        (L R : MM.mmap (exprs types)) (S : SUBST.Subst types) progress,
+        SUBST.Subst_WellTyped (typeof_funcs funcs) (typeof_env U) (typeof_env G) sub ->
+        SUBST.Subst_WellTyped (typeof_funcs funcs) (typeof_env U) (typeof_env G) S ->
+        SUBST.Subst_equations funcs U G S ->
+        Valid Prover_correct U G summ ->
+        SH.WellTyped_impures (typeof_funcs funcs) (typeof_preds preds)
+        (typeof_env U) (typeof_env G) acc = true ->
+        SH.WellTyped_impures (typeof_funcs funcs) (typeof_preds preds)
+        (typeof_env U) (typeof_env G) rem = true ->
+        forall P Q,
+          himp funcs preds U G
+          (Star (SH.impuresD (impuresInstantiate S R)) P)
+          (Star (SH.impuresD (impuresInstantiate S L)) Q) ->
+          forall p : predicate types,
+            nth_error preds n = Some p ->
+            all2 (is_well_typed (typeof_funcs funcs) (typeof_env U) (typeof_env G))
+            (map (SUBST.exprInstantiate S) e) (typeof_pred p) = true ->
+            allb
+            (fun v : list (expr types) * func =>
+              match nth_error (typeof_preds preds) (snd v) with
+                | Some ts =>
+                  all2
+                  (is_well_typed (typeof_funcs funcs) (typeof_env U) (typeof_env G))
+                  (map (SUBST.exprInstantiate S) (fst v)) ts
+                | None => false
+              end) ls = true ->
+            cancel_in_order bound summ (SE.typeof_preds preds) ls (MM.mmap_add n e acc) rem sub progress = Some (L, R, S) ->
+            himp funcs preds U G
+            (Star (SH.impuresD (impuresInstantiate S rem)) P)
+            (Star (Star
+              (SE.Star (Func n (map (SUBST.exprInstantiate S) e))
+                (SH.starred
+                  (fun v : list (expr types) * func =>
+                    Func (snd v) (map (SUBST.exprInstantiate S) (fst v))) ls Emp))
+              (SH.impuresD (impuresInstantiate S acc))) Q).
+    Proof.
+      intros. 
+      assert (allb (fun v : list (expr types) * func => WellTyped_sexpr (typeof_funcs funcs) (typeof_preds preds) 
+        (typeof_env U) (typeof_env G) (Func (snd v) (fst v))) ls = true).
+      { eapply allb_impl. eauto. simpl. intros. destruct (nth_error (typeof_preds preds) (snd x)); auto.
+        rewrite all2_map_1 in H11. eapply all2_impl; try eassumption. intros.
+        simpl in *. rewrite <- SUBST.exprInstantiate_WellTyped in H12; eauto. }
+      assert (SH.WellTyped_impures (typeof_funcs funcs) (typeof_preds preds)
+        (typeof_env U) (typeof_env G) (MM.mmap_add n e acc) = true).
+      { eapply WellTyped_impures_mmap_add. eauto. rewrite nth_error_typeof_preds. rewrite H7. simpl.
+        unfold typeof_pred. rewrite all2_map_1 in H8. eapply all2_impl. eauto. simpl.
+        intros. rewrite <- SUBST.exprInstantiate_WellTyped in H12; eauto. }
+      generalize H10. eapply cancel_in_order_PureFacts in H10; eauto. intro.
+      eapply H in H13; eauto. intuition.
+      rewrite H13.
+      do 2 rewrite SEP_UFACTS.impuresD_forget_impuresInstantiate by eassumption.
+      rewrite impuresD_mmap_add. rewrite Func_forget_exprInstantiate by eassumption.
+      rewrite heq_star_comm with (Q := SH.starred
+        (fun v : list (expr types) * func =>
+          Func (snd v) (map (SUBST.exprInstantiate S) (fst v))) ls Emp).
+      repeat rewrite heq_star_assoc. reflexivity.
+    Qed.
+
+    (** cancel_in_order ls acc rem = (l,r,sub) ->
+     ** r ===> l ->
+     ** rem ===> ls * acc
+     **)
+    Lemma cancel_in_orderOk : forall U G bound summ ls acc rem sub L R S progress,
+      let tf := typeof_funcs funcs in
+      let tp := SE.typeof_preds preds in
+      let tU := typeof_env U in
+      let tG := typeof_env G in
+      SUBST.Subst_WellTyped tf tU tG sub ->
+      SUBST.Subst_WellTyped tf tU tG S ->
+      SUBST.Subst_equations funcs U G S ->
+      Valid Prover_correct U G summ ->
+      cancel_in_order bound summ tp ls acc rem sub progress = Some (L, R, S) ->
+      allb (fun v => SE.WellTyped_sexpr tf tp tU tG 
+        (Func (snd v) (map (@SUBST.exprInstantiate _ S) (fst v)))) ls = true ->
+      SH.WellTyped_impures tf tp tU tG acc = true ->
+      SH.WellTyped_impures tf tp tU tG rem = true ->
+      forall P Q,
+      himp funcs preds U G 
+        (Star (SH.impuresD (impuresInstantiate S R)) P)
+        (Star (SH.impuresD (impuresInstantiate S L)) Q) ->
+      himp funcs preds U G 
+        (Star (SH.impuresD (impuresInstantiate S rem)) P)
+        (Star (Star (SH.starred (fun v => (Func (snd v) (map (@SUBST.exprInstantiate _ S) (fst v)))) ls Emp)
+                    (SH.impuresD (impuresInstantiate S acc))) Q).
+    Proof.
+      induction ls; simpl; intros.
+      { destruct progress; try congruence. inversion H3; clear H3; subst. 
+        repeat rewrite starred_nil. rewrite heq_star_emp_l. auto. }
+      { rewrite starred_cons. rewrite nth_error_typeof_preds in H4. destruct a; simpl in *.
+        repeat match goal with
+                 | H : context [ option_map _ ?X ] |- _ =>
+                   (consider X; simpl in *; try congruence); [ intros ]
+                 | [ H : match ?X with _ => _ end = _ |- _ ] =>
+                   (consider X; intros; try congruence); [ intros ]
+                 | [ H : match ?X with
+                           | Some _ => _ | None => _ 
+                         end = _ |- _ ] =>
+                 consider X; intros
+               end; simpl in *; subst.
+        { assert (all2 (is_well_typed (typeof_funcs funcs) (typeof_env U) (typeof_env G)) e (SDomain p) = true).
+          { rewrite all2_map_1 in H8. eapply all2_impl. eapply H8. intros. simpl in *.
+            rewrite <- SUBST.exprInstantiate_WellTyped in H11; eauto. }
+          assert (List.Forall (fun r : list (expr types) =>
+            all2 (is_well_typed (typeof_funcs funcs) (typeof_env U) (typeof_env G)) r (SDomain p) = true) l).
+          { eapply SH.WellTyped_impures_eq in H6; eauto. destruct l. constructor.
+            rewrite nth_error_typeof_preds in *. rewrite H4 in H6. revert H6.
+            generalize (e0 :: l). simpl. clear. induction l; simpl; intros; auto.
+            consider (all2 (is_well_typed (typeof_funcs funcs) (typeof_env U) (typeof_env G)) a (typeof_pred p)); intros.
+            constructor; auto. }
+          assert (t = SDomain p).
+          { clear - H4 H10. unfold typeof_preds, typeof_pred in *. rewrite map_nth_error_full in *.
+            rewrite H4 in *. inversion H10; auto. }
+          generalize H11. eapply unify_remove_PureFacts in H11. 
+          5: subst t; eassumption. 2: solve [ eauto ]. 2: solve [ eauto ].
+(* eauto using typeof_env_WellTyped_env, typeof_funcs_WellTyped_funcs. *)
+          intuition.
+          assert (allb (fun v : list (expr types) * func =>
+            WellTyped_sexpr (typeof_funcs funcs) (typeof_preds preds)
+            (typeof_env U) (typeof_env G) (Func (snd v) (fst v))) ls = true).
+          { eapply allb_impl. eassumption. simpl. intros.
+            destruct (nth_error (typeof_preds preds) (snd x)); auto.
+            rewrite all2_map_1 in H18. eapply all2_impl. eauto. simpl. intros.
+            rewrite <- SUBST.exprInstantiate_WellTyped in H20; eauto. }
+          assert (SH.WellTyped_impures (typeof_funcs funcs) (typeof_preds preds)
+            (typeof_env U) (typeof_env G) (FM.add n l0 rem) = true).
+          { eapply WellTyped_impures_add; eauto. 
+            rewrite nth_error_typeof_preds in *. rewrite H4. simpl. revert H19. clear.
+            unfold typeof_pred in *. induction 1; simpl; think; auto. }
+          Focus 2. eapply H14.
+          generalize H13. eapply cancel_in_order_PureFacts in H13; eauto.
+          intuition.
+          do 2 rewrite SEP_UFACTS.impuresD_forget_impuresInstantiate by eassumption.
+          assert (MM.PROPS.Add n l (FM.remove (elt:=list (exprs types)) n rem) rem).
+          { red. intro. rewrite MF.FACTS.add_o. rewrite MF.FACTS.remove_o.
+            destruct (MF.FACTS.eq_dec n y); subst; auto. }
+          assert (~FM.In (elt:=list (exprs types)) n (FM.remove (elt:=list (exprs types)) n rem)).
+          { rewrite MF.FACTS.remove_in_iff. intro. intuition; congruence. }
+          rewrite SH.impuresD_Add with (i := FM.remove n rem) (i' := rem) (f := n) (argss := l) by eassumption.
+          rewrite heq_star_assoc.          
+          rewrite Func_forget_exprInstantiate by eassumption.
+          subst t.
+          eapply unify_removeOk in H12; [ | | | | eassumption | | | | | | ];
+            eauto using typeof_env_WellTyped_env, typeof_funcs_WellTyped_funcs.
+          destruct H12. repeat rewrite heq_star_assoc. rewrite <- H12. rewrite heq_star_comm. rewrite <- SH.starred_base. 
+          reflexivity.
+          eapply IHls in H21; eauto.
+          do 2 rewrite SEP_UFACTS.impuresD_forget_impuresInstantiate in H21 by eassumption.
+          rewrite heq_star_assoc in H21. rewrite <- H21.
+          rewrite SH.impuresD_Add with (i := FM.remove n rem) (i' := FM.add n l0 rem) (f := n) (argss := l0).
+          rewrite SH.starred_base. rewrite heq_star_comm. rewrite heq_star_assoc. reflexivity.
+          { intro. repeat (rewrite MF.FACTS.add_o || rewrite MF.FACTS.remove_o). destruct (MF.FACTS.eq_dec n y); auto. }
+          { rewrite MF.FACTS.remove_in_iff. intro. intuition; congruence. } }
+        { eapply cancel_in_order_common in H12; eauto. }
+        { eapply cancel_in_order_common in H11; eauto. } 
+      { eapply cancel_in_order_common in H10; eauto. } }
+    Qed.
+
+
+    (** NOTE: return None if we don't make progress
+     **)
+    Definition sepCancel (bound : nat) (tpreds : SE.tpredicates) (summ : Facts Prover) (l r : SH.SHeap types) (s : SUBST.Subst types) 
+      : option (SH.SHeap _ * SH.SHeap _ * SUBST.Subst types) :=
+      let ordered_r := O.order_impures (SH.impures r) in
+      let sorted_l := FM.map (fun v => Ordering.sort _ (@O.meta_order_args _) v) (SH.impures l) in 
+      match 
+        cancel_in_order bound summ tpreds ordered_r (MM.empty _) sorted_l s false
+        with
+        | None => None 
+        | Some (rf, lf, sub) =>
+          Some ({| SH.impures := lf ; SH.pures := SH.pures l ; SH.other := SH.other l |},
+                {| SH.impures := rf ; SH.pures := SH.pures r ; SH.other := SH.other r |},
+                sub)
+      end.
+
+    Theorem sepCancel_PuresPrem : forall tp U G bound summ l r l' r' s s',
+      sepCancel bound tp summ l r s = Some (l', r', s') ->
+      AllProvable funcs U G (SH.pures l) ->
+      AllProvable funcs U G (SH.pures l').
+    Proof.
+      unfold sepCancel. intros.
+      destruct (cancel_in_order bound summ tp (O.order_impures (SH.impures r))
+              (MM.empty (exprs types))
+              (FM.map
+                 (fun v : list (exprs types) =>
+                  Ordering.sort (exprs types) (@O.meta_order_args _) v)
+                 (SH.impures l)) s). destruct p. destruct p. inversion H.
+      auto. congruence.
+    Qed.
+
+    Lemma starred_ext : forall T U G F F' (ls : list T) B,
+      (forall x, heq funcs preds U G (F x) (F' x)) -> 
+      heq funcs preds U G (SH.starred F ls B) (SH.starred F' ls B).
+    Proof. clear.
+      induction ls; intros; repeat (rewrite starred_nil || rewrite starred_cons).
+      reflexivity. rewrite H. rewrite IHls; auto. reflexivity.
+    Qed.
+
+    Lemma Equiv_map : forall T (E : T -> T -> Prop) (F : T -> T) a,
+      (forall x, E (F x) x) ->
+      FM.Equiv E (FM.map F a) a.
+    Proof. clear.
+      red; intros. split; intros.
+      rewrite MF.PROPS.F.map_in_iff. tauto.
+      apply MF.FACTS.map_mapsto_iff in H0. destruct H0. intuition; subst.
+      apply MF.FACTS.find_mapsto_iff in H1. apply MF.FACTS.find_mapsto_iff in H3. 
+      rewrite H1 in H3; inversion H3; auto.
+    Qed.
+
+
+    Lemma WellTyped_empty : forall tf tp tU tG,
+      SH.WellTyped_impures tf tp tU tG (MM.empty (exprs types)) = true.
+    Proof. clear.
+      intros. rewrite SH.WellTyped_impures_spec_eq. rewrite MF.PROPS.fold_Empty; auto with typeclass_instances.
+      apply FM.empty_1.
+    Qed.
+
+    
+
+    Lemma map_sort_WellTyped : forall C tf tp tU tG imp,
+      SH.WellTyped_impures tf tp tU tG imp = true ->
+      SH.WellTyped_impures tf tp tU tG
+      (FM.map (fun v : list (exprs types) => Ordering.sort (exprs types) C v) imp) = true.
+    Proof. clear.
+      intros. eapply SH.WellTyped_impures_eq; intros. rewrite MF.FACTS.map_o in H0.
+      consider (FM.find (elt:=list (exprs types)) k imp); simpl in *; try congruence; intros.
+      inversion H1; clear H1; subst.
+      eapply SH.WellTyped_impures_eq in H0. 2: eassumption.
+      destruct l; auto. destruct (nth_error tp k); try contradiction.
+      erewrite allb_permutation in H0. 2: symmetry; eapply Ordering.sort_permutation.
+      rewrite H0. destruct (Ordering.sort (exprs types) C (e :: l)); auto. 
+    Qed.
+
+    Theorem sepCancel_PureFacts : forall tU tG bound summ l r l' r' s s',
+      let tf := typeof_funcs funcs in
+      let tp := typeof_preds preds in
+      sepCancel bound tp summ l r s = Some (l', r', s') ->
+      SUBST.Subst_WellTyped tf tU tG s ->
+      SH.WellTyped_sheap tf tp tU tG l = true ->
+      SH.WellTyped_sheap tf tp tU tG r = true ->
+         SUBST.Subst_WellTyped tf tU tG s' 
+      /\ SH.WellTyped_sheap tf tp tU tG l' = true
+      /\ SH.WellTyped_sheap tf tp tU tG r' = true
+      /\ SUBST.Subst_Extends s' s.
+    Proof. 
+      unfold sepCancel. intros.
+      consider (cancel_in_order bound summ (typeof_preds preds) (O.order_impures (SH.impures r))
+              (MM.empty (exprs types))
+              (FM.map
+                 (fun v : list (exprs types) =>
+                  Ordering.sort (exprs types) (@O.meta_order_args _) v)
+                 (SH.impures l)) s false); intros.
+      destruct p. destruct p. inversion H3; clear H3; subst.
+      rewrite SH.WellTyped_sheap_eq in H1.
+      rewrite SH.WellTyped_sheap_eq in H2. think.
+      eapply cancel_in_order_PureFacts_weak in H; try eassumption; 
+        eauto using O.order_impures_WellTyped, WellTyped_empty, map_sort_WellTyped.
+      intuition.
+      rewrite SH.WellTyped_sheap_eq; simpl; think; auto.
+      rewrite SH.WellTyped_sheap_eq; simpl; think; auto.
+      congruence.
+    Qed.
+
+    Theorem sepCancel_correct : forall U G bound summ l r l' r' sub sub',
+      SUBST.Subst_WellTyped (typeof_funcs funcs) (typeof_env U) (typeof_env G) sub' ->
+      SH.WellTyped_sheap (typeof_funcs funcs) (typeof_preds preds) (typeof_env U) (typeof_env G) l = true ->
+      SH.WellTyped_sheap (typeof_funcs funcs) (typeof_preds preds) (typeof_env U) (typeof_env G) r = true ->
+      Valid Prover_correct U G summ ->
+      sepCancel bound (typeof_preds preds) summ l r sub' = Some (l', r', sub) ->
+      himp funcs preds U G (SH.sheapD l') (SH.sheapD r') ->
+      SUBST.Subst_equations funcs U G sub ->
+      himp funcs preds U G (SH.sheapD l) (SH.sheapD r).
+    Proof.
+      destruct l; destruct r. unfold sepCancel. simpl. intros.
+      repeat match goal with 
+               | [ H : match ?X with _ => _ end = _ |- _ ] => 
+                 revert H; case_eq X; intros; try congruence
+               | [ H : prod _ _ |- _ ] => destruct H
+               | [ H : (_,_) = (_,_) |- _ ] => inversion H; clear H; subst
+               | [ H : Some _ = Some _ |- _ ] => inversion H; clear H; subst
+             end.
+      do 2 rewrite SH.sheapD_def. simpl. 
+      eapply cancel_in_orderOk with (U := U) (G := G) 
+        (P := Star (SH.starred (@SE.Inj _) pures SE.Emp)
+                   (SH.starred (@SE.Const _) other SE.Emp)) 
+        (Q := Star (SH.starred (@SE.Inj _) pures0 SE.Emp)
+                   (SH.starred (@SE.Const _) other0 SE.Emp)) in H3;
+        eauto using typeof_env_WellTyped_env, typeof_funcs_WellTyped_funcs, SUBST.Subst_empty_WellTyped.
+      { clear H4.
+        do 2 rewrite impuresD_forget_impuresInstantiate in H3 by eassumption. 
+        rewrite SH.impuresD_Empty with (i := MM.empty _) in H3.
+        rewrite starred_ext with (ls := O.order_impures impures0) in H3. 2: intro; apply Func_forget_exprInstantiate; auto.
+        rewrite SH.impuresD_Equiv with (b := impures) in H3.
+        rewrite H3. repeat rewrite heq_star_assoc. apply himp_star_frame.
+        rewrite <- O.order_impures_D. reflexivity.
+        rewrite heq_star_emp_l. reflexivity.
+
+        red.
+        symmetry. erewrite Equiv_map. reflexivity. intros. eapply Ordering.sort_permutation.
+        apply FM.empty_1. }
+      { eapply SUBST.Subst_equations_WellTyped; auto. }
+      { rewrite SH.WellTyped_sheap_eq in H1. think. simpl in *.
+        eapply O.order_impures_WellTyped in H1.
+        eapply allb_impl; try eassumption. simpl; intros.
+        destruct (nth_error (typeof_preds preds) (snd x)); auto.
+        rewrite all2_map_1. erewrite all2_impl. 2: eauto. auto.        
+        simpl; intros.
+        rewrite <- SUBST.exprInstantiate_WellTyped; auto using SUBST.Subst_equations_WellTyped. }
+      { apply WellTyped_empty. }
+      { apply map_sort_WellTyped. rewrite SH.WellTyped_sheap_eq in H0. think. simpl in *. auto. }
+      { do 2 (rewrite SH.sheapD_def in H4; simpl in H4). 
+        do 2 rewrite impuresD_forget_impuresInstantiate by eassumption. eapply H4. }
+    Qed.
+
+  End env.
+
+End Make.
